translator/repl/ml_repl_stepScript.sml
@@ -6,30 +6,18 @@ val _ = new_theory "ml_repl_step";
 open repl_funTheory CompilerTheory CompilerLibTheory;
 open ToIntLangTheory ToBytecodeTheory terminationTheory ElabTheory;
 open compilerTerminationTheory inferTheory CompilerPrimitivesTheory;
-open BytecodeTheory;
+open BytecodeTheory mmlParseTheory mmlPEGTheory;
 
-open arithmeticTheory listTheory finite_mapTheory;
+open arithmeticTheory listTheory finite_mapTheory pred_setTheory;
 open ml_translatorLib ml_translatorTheory std_preludeTheory;
 
 val _ = translation_extends "std_prelude";
 
+(* translator setup *)
 
-
-(* types *)
-
-val _ = register_type ``:top``;     (* AstTheory *)
-val _ = register_type ``:ast_top``; (* ElabTheory *)
-val _ = register_type ``:Cexp``;    (* TntLangTheory *)
-val _ = register_type ``:bc_inst``; (* bytecode instruction *)
-val _ = register_type ``:compiler_state``;
-
-(* compiler *)
-
-val CCRef_expand =
-  prove(``CCRef = \x. CCRef x``, SIMP_TAC std_ss [FUN_EQ_THM]);
-
-val CTEnv_expand =
-  prove(``CTEnv = \x. CTEnv x``, SIMP_TAC std_ss [FUN_EQ_THM]);
+val lemma = prove(
+  ``(b <> [] /\ x) = if b = [] then F else x``,
+  Cases_on `b` THEN FULL_SIMP_TAC std_ss []);
 
 fun def_of_const tm = let
   val res = dest_thy_const tm
@@ -43,19 +31,67 @@ fun def_of_const tm = let
             def_from_thy "compilerTermination" name handle HOL_ERR _ =>
             def_from_thy (#Thy res) name handle HOL_ERR _ =>
             failwith ("Unable to find definition of " ^ name)
-  val def = def |> RW1 [CCRef_expand,CTEnv_expand]
-                |> RW [MEMBER_INTRO,MAP]
+  val def = def |> RW [MEMBER_INTRO,MAP]
                 |> CONV_RULE (DEPTH_CONV BETA_CONV)
+                |> SIMP_RULE bool_ss [IN_INSERT,NOT_IN_EMPTY] |> RW [lemma]
   in def end
 
 val _ = (find_def_for_const := def_of_const);
+
+(* compiler *)
+
+val _ = register_type ``:bc_inst``;
 
 val fapply_thm = prove(
   ``fapply d x f = case FLOOKUP f x of NONE => d | SOME y => y``,
   SRW_TAC [] [fapply_def,FLOOKUP_DEF]);
 
 val _ = translate fapply_thm;
-val _ = translate compile_top_def;
+val _ = translate compile_dec_def;
+(* val _ = translate compile_top_def; *)
 
+(* parser *)
+
+val _ = (find_def_for_const := (fn _ => fail()));
+
+(* It's really confusing that mmlPEG and mmlParse define
+   different splitAt functions *)
+val _ = translate mmlPEGTheory.splitAt_def;
+val _ = translate FUPDATE_LIST;
+val _ = translate (def_of_const ``pnt``);
+val _ = translate (def_of_const ``sumID``);
+val _ = translate (def_of_const ``bindNT``);
+val _ = translate (def_of_const ``mktokLf``);
+val _ = translate (def_of_const ``destSymbolT``);
+val _ = translate (def_of_const ``destAlphaT``);
+val _ = translate (def_of_const ``OPTION_BIND``);
+val _ = translate (def_of_const ``isUpper``);
+val _ = translate (def_of_const ``assert``);
+val _ = translate (def_of_const ``peg_V``);
+val _ = translate (def_of_const ``pegf``);
+val _ = translate (def_of_const ``seql``);
+val _ = translate (def_of_const ``destLongidT``);
+val _ = translate (def_of_const ``isLower``);
+val _ = translate (def_of_const ``isAlpha``);
+val _ = translate (def_of_const ``peg_longV``);
+val _ = translate (def_of_const ``peg_Eapp``);
+val _ = translate (def_of_const ``tokeq``);
+val _ = translate (def_of_const ``isInt``);
+val _ = translate (def_of_const ``isLongidT``);
+val _ = translate (def_of_const ``isTyvarT``);
+val _ = translate (def_of_const ``choicel``);
+val _ = translate (def_of_const ``mk_linfix``);
+val _ = translate (def_of_const ``peg_linfix``);
+val _ = translate (def_of_const ``peg_nonfix``);
+val _ = translate (def_of_const ``try``);
+val _ = translate (def_of_const ``peg_Type``);
+val _ = translate (def_of_const ``mk_rinfix``);
+val _ = translate (def_of_const ``isAlphaSym``);
+val _ = translate (def_of_const ``calcTyOp``);
+val _ = translate (def_of_const ``peg_DType``);
+val _ = translate (def_of_const ``peg_TypeName``);
+val _ = translate (def_of_const ``peg_TypeDec``);
+val _ = translate (def_of_const ``peg_UQConstructorName``);
+val _ = translate (def_of_const ``mmlPEG``);
 
 val _ = export_theory();
